theories/VLSM/Core/Equivocators/Composition/LimitedEquivocation/FixedEquivocation.v
@@ -1308,7 +1308,7 @@ Proof.
     remember (pre_VLSM_projection_finite_trace_project _ _ _ _ _) as tr.
     replace tr with (equivocators_total_trace_project IM trX); [done |].
     subst. symmetry.
-    apply (equivocators_total_VLSM_projection_trace_project IM (proj1 Hpre_tr)).
+    apply (equivocators_total_VLSM_projection_finite_trace_project IM (proj1 Hpre_tr)).
 Qed.
 
 End from_equivocators_to_nodes.
